ρ₁_initial 의 증명에서 cbv 를 simp 로 변경 - 증명이 더 깔끔해졌네! - ...근데 simp가 많아져서, 좀 느려진 것 같기도;;

Nemonuri/Executions/ExecutionFragment/Expr/Raw.lean
@@ -125,24 +125,6 @@ theorem stepL'_preserves_label {s a} : HasLabel.Preserves Label (@stepL' ts s a)
 theorem stepL'_preserves_seqLabel {s a} : HasLabel.Preserves Sequence.Label (@stepL' ts s a) := @stepL_preserves_seqLabel ts s a
 
 
-def pre : ExprRaw ts → ts.FiniteExecutionFragmentRaw
-  | .finite1 total => total
-  | .finite2 pre _ => pre
-  | .infinite1 pre => pre
-
-section Pre
-
-@[defeq, simp]
-theorem finite1_pre {x} : (@ExprRaw.finite1 ts x).pre = x := rfl
-
-@[defeq, simp]
-theorem finite2_pre {x1 x2} : (@ExprRaw.finite2 ts x1 x2).pre = x1 := rfl
-
-@[defeq, simp]
-theorem infinite1_pre {x} : (@ExprRaw.infinite1 ts x).pre = x := rfl
-
-end Pre
-
 
 def post (ex: ExprRaw ts) (req: ex.toSeqLabel = .finite) : ts.FiniteExecutionFragmentRaw :=
   match ex with
@@ -159,10 +141,6 @@ theorem finite1_post {x} : (@ExprRaw.finite1 ts x).post finite1_toSeqLabel = x :
 theorem finite2_post {x1 x2} : (@ExprRaw.finite2 ts x1 x2).post finite2_toSeqLabel = x2 := rfl
 
 end Post
-
-
-theorem stepL_pre_eq_pre_stepL {tail s a} : (@stepL ts tail s a).pre = (tail.pre.stepL s a) := by
-  cases tail <;> rfl
 
 
 
