Nemonuri/Executions/ExecutionFragment/Expr/Pre.lean
@@ -1,0 +1,76 @@
+module
+
+public import Nemonuri.Executions.ExecutionFragment.Expr.Raw
+
+@[expose] public section
+
+namespace Nemonuri.TransitionSystem.ExecutionFragment.ExprRaw
+
+variable {ts: TransitionSystem}
+
+
+def pre : ExprRaw ts → ts.FiniteExecutionFragmentRaw
+  | .finite1 total => total
+  | .finite2 pre _ => pre
+  | .infinite1 pre => pre
+
+
+
+@[defeq, simp]
+theorem finite1_pre {x} : (@ExprRaw.finite1 ts x).pre = x := rfl
+
+@[defeq, simp]
+theorem finite2_pre {x1 x2} : (@ExprRaw.finite2 ts x1 x2).pre = x1 := rfl
+
+@[defeq, simp]
+theorem infinite1_pre {x} : (@ExprRaw.infinite1 ts x).pre = x := rfl
+
+@[defeq, simp]
+theorem singleState_pre_states {s} : (@singleState ts s).pre.states = [s] := rfl
+
+@[defeq, simp]
+theorem singleState_pre_actions {s} : (@singleState ts s).pre.actions = [] := rfl
+
+@[defeq, simp]
+theorem ellipsis_pre_states : (@ellipsis ts).pre.states = [] := rfl
+
+@[defeq, simp]
+theorem ellipsis_pre_actions : (@ellipsis ts).pre.actions = [] := rfl
+
+@[simp]
+theorem consEllipsis_pre_states {x} (req: x.toLabel = .finite1) : (@consEllipsis ts x).pre.states = [] := by
+  cases x <;> simp at req
+  · rfl
+
+@[simp]
+theorem consEllipsis_pre_actions {x} (req: x.toLabel = .finite1) : (@consEllipsis ts x).pre.actions = [] := by
+  cases x <;> simp at req
+  · rfl
+
+section StepL
+
+variable {tail: ExprRaw ts} {s: ts.S} {a: ts.Act}
+
+theorem stepL_pre_eq_pre_stepL : (stepL tail s a).pre = (tail.pre.stepL s a) := by
+  cases tail <;> rfl
+
+@[simp]
+theorem stepL_pre_states_eq_pre_stepL_states : (stepL tail s a).pre.states = (tail.pre.stepL s a).states :=
+  congrArg FiniteExecutionFragmentRaw.states stepL_pre_eq_pre_stepL
+
+@[simp]
+theorem stepL_pre_actions_eq_pre_stepL_actions : (stepL tail s a).pre.actions = (tail.pre.stepL s a).actions :=
+  congrArg FiniteExecutionFragmentRaw.actions stepL_pre_eq_pre_stepL
+
+end StepL
+
+--theorem stepL_pre_states
+
+
+
+
+
+
+end Nemonuri.TransitionSystem.ExecutionFragment.ExprRaw
+
+end
