Nemonuri/Executions/FiniteExecutionFragment/Raw.lean
@@ -20,6 +20,18 @@ def singleState (s: ts.S) : ts.FiniteExecutionFragmentRaw := ⟨[s], []⟩
 def stepL (tail: ts.FiniteExecutionFragmentRaw) (state0: ts.S) (action0: ts.Act) : ts.FiniteExecutionFragmentRaw :=
   ⟨state0 :: tail.states, action0 :: tail.actions⟩
 
+section StepL
+
+variable {tl: ts.FiniteExecutionFragmentRaw} {s0: ts.S} {a0: ts.Act}
+
+@[defeq, simp]
+theorem stepL_states : (tl.stepL s0 a0).states = s0 :: tl.states := rfl
+
+@[defeq, simp]
+theorem stepL_actions : (tl.stepL s0 a0).actions = a0 :: tl.actions := rfl
+
+end StepL
+
 
 end FiniteExecutionFragmentRaw
 
